coq/lang/TriplesGraphs.v
@@ -1,0 +1,117 @@
+Set Implicit Arguments.
+From Lang Require Export Assertions.
+
+Implicit Type m : mem.
+Implicit Type n : int.
+Implicit Type I : binding.
+Implicit Type c : cmd.
+
+
+Inductive stmt : Type :=
+| StmtTriple (c:cmd) (P Q : assrt)
+| StmtAssrt (P:assrt).
+
+
+Notation "'|-' c ':' P '=>' Q" := 
+  (StmtTriple c P%A Q%A)
+  (at level 50, c at next level, no associativity).
+
+Notation "'|-' P" :=
+  (StmtAssrt P%A)
+  (at level 50, no associativity).
+
+
+(*Section Graphs.
+
+  Variable rule : Type.
+
+  Variable ruleID : rule.
+
+  Definition nodeID := nat.
+
+  Definition node : Type := 
+    nodeID * stmt * rule * list nodeID.
+
+  Definition graph := fmap nodeID node.
+
+  Definition node_dummy : node := (O,|-true,ruleID,[]).
+
+  Global Instance Inhab_node : Inhab node.
+  Proof using ruleID.
+    constructor. exists~ node_dummy.
+  Qed.
+
+  Variable is_rule_instance : graph -> node -> Prop.
+
+End Graphs.*)
+
+
+
+Inductive rule :=
+| HL_CSQ
+| HL_Case
+| HL_Skip
+| HL_Assn
+| HL_Seq
+| HL_IfTrue
+| HL_IfFalse
+| HL_WhileTrue
+| HL_WhileFalse
+| HL_AssrtLift.
+
+Definition nodeID := nat.
+
+Definition node : Type := 
+  nodeID * stmt * rule * list nodeID.
+
+Definition graph := fmap nodeID node.
+
+Definition node_dummy : node := (O,|-true,HL_Seq,[]).
+
+Global Instance Inhab_node : Inhab node.
+Proof using.
+  constructor. exists~ node_dummy.
+Qed.
+
+Inductive is_rule_instance (g:graph) : node -> Prop :=
+  | Rule_HL_CSQ nid id1 id2 id3 P P' Q Q' c r1 r2 r3 prems1 prems2 prems3
+    (H1 : read g id1 = (id1,|- (P->P'),r1,prems1)) 
+    (H2 : read g id2 = (id2,|- c : P' => Q',r2,prems2))
+    (H3 : read g id3 = (id3,|- (Q'->Q),r3,prems3))
+    : is_rule_instance g (nid,|- c : P => Q,HL_CSQ,[id1;id2;id3])
+
+  | Rule_HL_Case nid id1 id2 P P' Q c r1 r2 prems1 prems2
+    (H1 : read g id1 = (id1,|- c : P /\ P' => Q,r1,prems1))
+    (H2 : read g id2 = (id2,|- c : P /\ ~ P' => Q,r2,prems2))
+    : is_rule_instance g (nid,|- c : P => Q,HL_Case,[id1;id2])
+
+  | Rule_HL_Skip nid P
+    : is_rule_instance g (nid,|- CSkip : P => P,HL_Skip,[])
+
+  | Rule_HL_Assn nid x a P
+    : is_rule_instance g (nid,|- CAssn x a : P[a/x] => P,HL_Assn,[])
+
+  | Rule_HL_Seq nid id1 id2 P Q R c1 c2 r1 r2 prems1 prems2
+    (H1 : read g id1 = (id1, |- c1 : P => Q, r1, prems1))
+    (H2 : read g id2 = (id2, |- c2 : Q => R, r2, prems2))
+    : is_rule_instance g (nid, |- CSeq c1 c2 : P => R, HL_Seq, [id1;id2])
+  
+  | Rule_HL_IfTrue nid id1 P Q (b:bexp) c c' r1 prems1
+    (H1 : read g id1 = (id1, |- c : P /\ b => Q, r1, prems1))
+    : is_rule_instance g (nid, |- CIf b c c' : P /\ b => Q, HL_IfTrue, [id1]%list)
+
+  | Rule_HL_IfFalse nid id1 P Q (b:bexp) c c' r1 prems1
+    (H1 : read g id1 = (id1, |- c' : P /\ ~b => Q, r1, prems1))
+    : is_rule_instance g (nid, |- CIf b c c' : P /\ ~b => Q, HL_IfFalse, [id1]%list)
+
+  | Rule_HL_WhileTrue nid id1 P Q (b:bexp) c r1 prems1
+    (H : read g id1 = (id1, |- CSeq c (CWhile b c) : P /\ b => Q, r1, prems1))
+    : is_rule_instance g (nid, |- CWhile b c : P /\ b => (Q /\ ~b), HL_WhileTrue, [id1]%list)
+
+  | Rule_HL_WhileFalse nid P b c
+    : is_rule_instance g (nid, |- CWhile b c : P /\ ~b => (P /\ ~b), HL_WhileFalse, [])
+
+  | Rule_AssrtLift nid P
+    (H : (|= P)%V)
+    : is_rule_instance g (nid, |- P, HL_AssrtLift, [])
+.
